theory/x64DecodeProof.thy
@@ -143,85 +143,36 @@ lemma x64_encode_decode_consistency:
   "list_in_list l_bin pc l \<Longrightarrow> Some l_bin = x64_encode ins \<Longrightarrow>
     x64_decode pc l = Some (length l_bin, ins)"
   apply (cases ins; simp_all)
-                      prefer 20
-  subgoal for addr imm chunk
-  \<comment> \<open> Paddq_mi \<close> 
-    apply (cases chunk, simp_all)
-    apply (cases addr)
-    subgoal for base index2 ofs
-      apply simp
-      apply (cases base, simp_all)
-      subgoal for base_reg
-        apply (cases index2, simp_all)
-        subgoal for index22
-          apply (cases index22, simp_all)
-          subgoal for index_reg scale
-            apply (erule conjE; erule conjE; erule conjE; erule conjE)
-            apply (simp add: list_in_list_concat; erule conjE)
 
-            using construct_modsib_to_u8_imply_index_reg [of index_reg base_reg "l ! pc" scale "l ! Suc (Suc (Suc pc))"]
-            using construct_modsib_to_u8_imply_base_reg [of index_reg base_reg "l ! pc" scale "l ! Suc (Suc (Suc pc))"]
-            using construct_modsib_to_u8_imply_scale [of scale index_reg base_reg "l ! (pc+3)"]
-            using list_in_list_u8_list_of_u32_simp_sym [of "ofs" "(pc+4)" l]
-            using length_u8_list_of_u32_eq_4
-            using list_in_list_u8_list_of_u32_simp_sym [of imm "(pc+8)" l]
-(*
-            apply (cases base_reg; simp; cases index_reg; simp add: construct_rex_to_u8_def construct_modsib_to_u8_def
-                    x64_decode_def bitfield_insert_u8_def Let_def ireg_of_u8_def
-                    add.commute Suc3_eq_add_3 Suc4_eq_add_4) *)
-            apply (cases base_reg; simp)
-            subgoal by (cases index_reg; simp add: construct_rex_to_u8_def construct_modsib_to_u8_def
-                    x64_decode_def bitfield_insert_u8_def Let_def ireg_of_u8_def
-                    add.commute Suc3_eq_add_3 Suc4_eq_add_4)
-            subgoal by (cases index_reg; simp add: construct_rex_to_u8_def construct_modsib_to_u8_def
-                    x64_decode_def bitfield_insert_u8_def Let_def ireg_of_u8_def
-                    add.commute Suc3_eq_add_3 Suc4_eq_add_4)
-            subgoal by (cases index_reg; simp add: construct_rex_to_u8_def construct_modsib_to_u8_def
-                    x64_decode_def bitfield_insert_u8_def Let_def ireg_of_u8_def
-                    add.commute Suc3_eq_add_3 Suc4_eq_add_4)
-            subgoal by (cases index_reg; simp add: construct_rex_to_u8_def construct_modsib_to_u8_def
-                    x64_decode_def bitfield_insert_u8_def Let_def ireg_of_u8_def
-                    add.commute Suc3_eq_add_3 Suc4_eq_add_4)
-            subgoal by (cases index_reg; simp add: construct_rex_to_u8_def construct_modsib_to_u8_def
-                    x64_decode_def bitfield_insert_u8_def Let_def ireg_of_u8_def
-                    add.commute Suc3_eq_add_3 Suc4_eq_add_4)
-            subgoal by (cases index_reg; simp add: construct_rex_to_u8_def construct_modsib_to_u8_def
-                    x64_decode_def bitfield_insert_u8_def Let_def ireg_of_u8_def
-                    add.commute Suc3_eq_add_3 Suc4_eq_add_4)
-            subgoal by (cases index_reg; simp add: construct_rex_to_u8_def construct_modsib_to_u8_def
-                    x64_decode_def bitfield_insert_u8_def Let_def ireg_of_u8_def
-                    add.commute Suc3_eq_add_3 Suc4_eq_add_4)
-            subgoal by (cases index_reg; simp add: construct_rex_to_u8_def construct_modsib_to_u8_def
-                    x64_decode_def bitfield_insert_u8_def Let_def ireg_of_u8_def
-                    add.commute Suc3_eq_add_3 Suc4_eq_add_4)
-            subgoal by (cases index_reg; simp add: construct_rex_to_u8_def construct_modsib_to_u8_def
-                    x64_decode_def bitfield_insert_u8_def Let_def ireg_of_u8_def
-                    add.commute Suc3_eq_add_3 Suc4_eq_add_4)
-            subgoal by (cases index_reg; simp add: construct_rex_to_u8_def construct_modsib_to_u8_def
-                    x64_decode_def bitfield_insert_u8_def Let_def ireg_of_u8_def
-                    add.commute Suc3_eq_add_3 Suc4_eq_add_4)
-            subgoal by (cases index_reg; simp add: construct_rex_to_u8_def construct_modsib_to_u8_def
-                    x64_decode_def bitfield_insert_u8_def Let_def ireg_of_u8_def
-                    add.commute Suc3_eq_add_3 Suc4_eq_add_4)
-            subgoal by (cases index_reg; simp add: construct_rex_to_u8_def construct_modsib_to_u8_def
-                    x64_decode_def bitfield_insert_u8_def Let_def ireg_of_u8_def
-                    add.commute Suc3_eq_add_3 Suc4_eq_add_4)
-            subgoal by (cases index_reg; simp add: construct_rex_to_u8_def construct_modsib_to_u8_def
-                    x64_decode_def bitfield_insert_u8_def Let_def ireg_of_u8_def
-                    add.commute Suc3_eq_add_3 Suc4_eq_add_4)
-            subgoal by (cases index_reg; simp add: construct_rex_to_u8_def construct_modsib_to_u8_def
-                    x64_decode_def bitfield_insert_u8_def Let_def ireg_of_u8_def
-                    add.commute Suc3_eq_add_3 Suc4_eq_add_4)
-            subgoal by (cases index_reg; simp add: construct_rex_to_u8_def construct_modsib_to_u8_def
-                    x64_decode_def bitfield_insert_u8_def Let_def ireg_of_u8_def
-                    add.commute Suc3_eq_add_3 Suc4_eq_add_4)
-            subgoal by (cases index_reg; simp add: construct_rex_to_u8_def construct_modsib_to_u8_def
-                    x64_decode_def bitfield_insert_u8_def Let_def ireg_of_u8_def
-                    add.commute Suc3_eq_add_3 Suc4_eq_add_4)
-            done
-          done
-        done
+                      prefer 61
+  subgoal for dst imm
+  \<comment> \<open> Ptestl_ri  \<close>
+    apply (unfold Let_def)
+    apply (cases "construct_rex_to_u8 False False False (and (u8_of_ireg dst) 8 \<noteq> 0) = 64";
+        simp_all add:construct_rex_to_u8_def construct_modsib_to_u8_def; erule conjE)
+    subgoal \<comment> \<open> rex = 0x40  \<close>
+      using list_in_list_u8_list_of_u32_simp_sym [of imm "(Suc (Suc pc))" l]
+      using length_u8_list_of_u32_eq_4
+      apply (cases dst; auto simp add: x64_decode_def bitfield_insert_u8_def Let_def
+          ireg_of_u8_def Suc3_eq_add_3 add.commute)
       done
+
+    subgoal \<comment> \<open> rex <> 0x40  \<close>
+      using list_in_list_u8_list_of_u32_simp_sym [of imm "(pc+3)" l]
+      using length_u8_list_of_u32_eq_4
+      apply (cases dst; auto simp add: x64_decode_def bitfield_insert_u8_def Let_def
+          ireg_of_u8_def Suc3_eq_add_3 add.commute)
+      done
+    done
+
+
+                      prefer 61
+  subgoal for dst imm
+  \<comment> \<open> Ptestq_ri  \<close>
+    apply (unfold Let_def construct_rex_to_u8_def construct_modsib_to_u8_def)
+    using list_in_list_u8_list_of_u32_simp_sym [of imm "(Suc (Suc (Suc pc)))" l]
+    using length_u8_list_of_u32_eq_4
+    apply (cases dst; simp_all add: bitfield_insert_u8_def x64_decode_def ireg_of_u8_def Suc3_eq_add_3 add.commute)
     done
 
 (*proof done
@@ -351,6 +302,86 @@ lemma x64_encode_decode_consistency:
   subgoal for dst imm 
     \<comment> \<open> Paddl_ri \<close> 
     sorry
+
+  subgoal for addr imm chunk
+  \<comment> \<open> Paddq_mi \<close> 
+    apply (cases chunk, simp_all)
+    apply (cases addr)
+    subgoal for base index2 ofs
+      apply simp
+      apply (cases base, simp_all)
+      subgoal for base_reg
+        apply (cases index2, simp_all)
+        subgoal for index22
+          apply (cases index22, simp_all)
+          subgoal for index_reg scale
+            apply (erule conjE; erule conjE; erule conjE; erule conjE)
+            apply (simp add: list_in_list_concat; erule conjE)
+
+            using construct_modsib_to_u8_imply_index_reg [of index_reg base_reg "l ! pc" scale "l ! Suc (Suc (Suc pc))"]
+            using construct_modsib_to_u8_imply_base_reg [of index_reg base_reg "l ! pc" scale "l ! Suc (Suc (Suc pc))"]
+            using construct_modsib_to_u8_imply_scale [of scale index_reg base_reg "l ! (pc+3)"]
+            using list_in_list_u8_list_of_u32_simp_sym [of "ofs" "(pc+4)" l]
+            using length_u8_list_of_u32_eq_4
+            using list_in_list_u8_list_of_u32_simp_sym [of imm "(pc+8)" l]
+(*
+            apply (cases base_reg; simp; cases index_reg; simp add: construct_rex_to_u8_def construct_modsib_to_u8_def
+                    x64_decode_def bitfield_insert_u8_def Let_def ireg_of_u8_def
+                    add.commute Suc3_eq_add_3 Suc4_eq_add_4) *)
+            apply (cases base_reg; simp)
+            subgoal by (cases index_reg; simp add: construct_rex_to_u8_def construct_modsib_to_u8_def
+                    x64_decode_def bitfield_insert_u8_def Let_def ireg_of_u8_def
+                    add.commute Suc3_eq_add_3 Suc4_eq_add_4)
+            subgoal by (cases index_reg; simp add: construct_rex_to_u8_def construct_modsib_to_u8_def
+                    x64_decode_def bitfield_insert_u8_def Let_def ireg_of_u8_def
+                    add.commute Suc3_eq_add_3 Suc4_eq_add_4)
+            subgoal by (cases index_reg; simp add: construct_rex_to_u8_def construct_modsib_to_u8_def
+                    x64_decode_def bitfield_insert_u8_def Let_def ireg_of_u8_def
+                    add.commute Suc3_eq_add_3 Suc4_eq_add_4)
+            subgoal by (cases index_reg; simp add: construct_rex_to_u8_def construct_modsib_to_u8_def
+                    x64_decode_def bitfield_insert_u8_def Let_def ireg_of_u8_def
+                    add.commute Suc3_eq_add_3 Suc4_eq_add_4)
+            subgoal by (cases index_reg; simp add: construct_rex_to_u8_def construct_modsib_to_u8_def
+                    x64_decode_def bitfield_insert_u8_def Let_def ireg_of_u8_def
+                    add.commute Suc3_eq_add_3 Suc4_eq_add_4)
+            subgoal by (cases index_reg; simp add: construct_rex_to_u8_def construct_modsib_to_u8_def
+                    x64_decode_def bitfield_insert_u8_def Let_def ireg_of_u8_def
+                    add.commute Suc3_eq_add_3 Suc4_eq_add_4)
+            subgoal by (cases index_reg; simp add: construct_rex_to_u8_def construct_modsib_to_u8_def
+                    x64_decode_def bitfield_insert_u8_def Let_def ireg_of_u8_def
+                    add.commute Suc3_eq_add_3 Suc4_eq_add_4)
+            subgoal by (cases index_reg; simp add: construct_rex_to_u8_def construct_modsib_to_u8_def
+                    x64_decode_def bitfield_insert_u8_def Let_def ireg_of_u8_def
+                    add.commute Suc3_eq_add_3 Suc4_eq_add_4)
+            subgoal by (cases index_reg; simp add: construct_rex_to_u8_def construct_modsib_to_u8_def
+                    x64_decode_def bitfield_insert_u8_def Let_def ireg_of_u8_def
+                    add.commute Suc3_eq_add_3 Suc4_eq_add_4)
+            subgoal by (cases index_reg; simp add: construct_rex_to_u8_def construct_modsib_to_u8_def
+                    x64_decode_def bitfield_insert_u8_def Let_def ireg_of_u8_def
+                    add.commute Suc3_eq_add_3 Suc4_eq_add_4)
+            subgoal by (cases index_reg; simp add: construct_rex_to_u8_def construct_modsib_to_u8_def
+                    x64_decode_def bitfield_insert_u8_def Let_def ireg_of_u8_def
+                    add.commute Suc3_eq_add_3 Suc4_eq_add_4)
+            subgoal by (cases index_reg; simp add: construct_rex_to_u8_def construct_modsib_to_u8_def
+                    x64_decode_def bitfield_insert_u8_def Let_def ireg_of_u8_def
+                    add.commute Suc3_eq_add_3 Suc4_eq_add_4)
+            subgoal by (cases index_reg; simp add: construct_rex_to_u8_def construct_modsib_to_u8_def
+                    x64_decode_def bitfield_insert_u8_def Let_def ireg_of_u8_def
+                    add.commute Suc3_eq_add_3 Suc4_eq_add_4)
+            subgoal by (cases index_reg; simp add: construct_rex_to_u8_def construct_modsib_to_u8_def
+                    x64_decode_def bitfield_insert_u8_def Let_def ireg_of_u8_def
+                    add.commute Suc3_eq_add_3 Suc4_eq_add_4)
+            subgoal by (cases index_reg; simp add: construct_rex_to_u8_def construct_modsib_to_u8_def
+                    x64_decode_def bitfield_insert_u8_def Let_def ireg_of_u8_def
+                    add.commute Suc3_eq_add_3 Suc4_eq_add_4)
+            subgoal by (cases index_reg; simp add: construct_rex_to_u8_def construct_modsib_to_u8_def
+                    x64_decode_def bitfield_insert_u8_def Let_def ireg_of_u8_def
+                    add.commute Suc3_eq_add_3 Suc4_eq_add_4)
+            done
+          done
+        done
+      done
+    done
 
   subgoal for dst src 
     \<comment> \<open> Psubl_rr \<close> 
@@ -492,5 +523,135 @@ lemma x64_encode_decode_consistency:
     apply (unfold Let_def construct_rex_to_u8_def construct_modsib_to_u8_def)
     apply (cases dst; auto simp add: x64_decode_def bitfield_insert_u8_def Let_def ireg_of_u8_def)
     done
+
+  subgoal for dst
+  \<comment> \<open> Pshlq_r \<close> 
+    apply (unfold Let_def construct_rex_to_u8_def construct_modsib_to_u8_def)
+    apply (cases dst; auto simp add: x64_decode_def bitfield_insert_u8_def Let_def ireg_of_u8_def)
+    done
+
+  subgoal for dst imm
+    \<comment> \<open> Pshrl_ri \<close>
+    apply (unfold Let_def)
+    apply (cases "construct_rex_to_u8 False False False (and (u8_of_ireg dst) 8 \<noteq> 0) = 64",
+        simp_all)
+
+    subgoal \<comment> \<open> rex = 0x40 \<close>
+      apply (cases dst; auto simp add: x64_decode_def bitfield_insert_u8_def Let_def ireg_of_u8_def
+          construct_rex_to_u8_def construct_modsib_to_u8_def)
+      done
+
+    subgoal  \<comment> \<open> rex <> 0x40 \<close>
+      apply (cases dst; auto simp add: x64_decode_def bitfield_insert_u8_def Let_def ireg_of_u8_def
+          construct_rex_to_u8_def construct_modsib_to_u8_def Suc3_eq_add_3 add.commute)
+      done
+    done
+
+  subgoal for dst
+    \<comment> \<open> Pshrq_ri \<close>
+    apply (unfold Let_def construct_rex_to_u8_def construct_modsib_to_u8_def; erule conjE; erule conjE)
+    apply (cases dst; auto simp add: x64_decode_def bitfield_insert_u8_def Let_def ireg_of_u8_def  Suc3_eq_add_3 add.commute)
+    done
+
+
+  subgoal for dst
+  \<comment> \<open> Pshrl_r \<close> 
+    apply (unfold Let_def construct_rex_to_u8_def construct_modsib_to_u8_def)
+    apply (cases dst; auto simp add: x64_decode_def bitfield_insert_u8_def Let_def ireg_of_u8_def)
+    done     
+
+  subgoal for dst
+  \<comment> \<open> Pshrq_r \<close> 
+    apply (unfold Let_def construct_rex_to_u8_def construct_modsib_to_u8_def)
+    apply (cases dst; auto simp add: x64_decode_def bitfield_insert_u8_def Let_def ireg_of_u8_def)
+    done
+
+  subgoal for dst imm
+    \<comment> \<open> Psarl_ri \<close>
+    apply (unfold Let_def construct_rex_to_u8_def construct_modsib_to_u8_def)
+    apply (cases dst; auto simp add: x64_decode_def bitfield_insert_u8_def Let_def ireg_of_u8_def  Suc3_eq_add_3 add.commute)
+    done
+
+  subgoal for dst
+  \<comment> \<open> Psarq_ri \<close> 
+    apply (unfold Let_def construct_rex_to_u8_def construct_modsib_to_u8_def; erule conjE; erule conjE)
+    apply (cases dst; auto simp add: x64_decode_def bitfield_insert_u8_def Let_def ireg_of_u8_def  Suc3_eq_add_3 add.commute)
+    done
+
+  subgoal for dst
+  \<comment> \<open> Psarl_r \<close> 
+    apply (unfold Let_def construct_rex_to_u8_def construct_modsib_to_u8_def)
+    apply (cases dst; auto simp add: x64_decode_def bitfield_insert_u8_def Let_def ireg_of_u8_def)
+    done  
+
+  subgoal for dst
+  \<comment> \<open> Psarq_r \<close> 
+    apply (unfold Let_def construct_rex_to_u8_def construct_modsib_to_u8_def)
+    apply (cases dst; auto simp add: x64_decode_def bitfield_insert_u8_def Let_def ireg_of_u8_def)
+    done  
+
+  subgoal for dst imm
+    \<comment> \<open> Prolw_ri \<close>
+    apply (unfold Let_def)
+    apply (cases "construct_rex_to_u8 False False False (and (u8_of_ireg dst) 8 \<noteq> 0) = 64",
+        simp_all)
+
+    subgoal \<comment> \<open> rex = 0x40 \<close>
+      apply (cases dst; auto simp add: x64_decode_def bitfield_insert_u8_def Let_def ireg_of_u8_def
+          construct_rex_to_u8_def construct_modsib_to_u8_def Suc3_eq_add_3 add.commute)
+      done
+
+    subgoal  \<comment> \<open> rex <> 0x40 \<close>
+      apply (cases dst; auto simp add: x64_decode_def bitfield_insert_u8_def Let_def ireg_of_u8_def
+          construct_rex_to_u8_def construct_modsib_to_u8_def Suc3_eq_add_3 add.commute)
+      done
+    done
+
+  subgoal for dst
+    \<comment> \<open> Pbswapl \<close> 
+    apply (unfold Let_def construct_rex_to_u8_def construct_modsib_to_u8_def)
+    subgoal by (cases dst; auto simp add: x64_decode_def bitfield_insert_u8_def Let_def ireg_of_u8_def)
+    done
+
+  subgoal for dst
+    \<comment> \<open> Pbswapq \<close> 
+    apply (unfold Let_def construct_rex_to_u8_def construct_modsib_to_u8_def)
+    subgoal by (cases dst; auto simp add: x64_decode_def bitfield_insert_u8_def Let_def ireg_of_u8_def)
+    done
+
+  subgoal for dst
+    \<comment> \<open> Ppushl_r \<close> 
+    apply (unfold Let_def construct_rex_to_u8_def construct_modsib_to_u8_def)
+    subgoal by (cases dst; auto simp add: x64_decode_def bitfield_insert_u8_def Let_def ireg_of_u8_def)
+    done
+
+  subgoal for imm
+    \<comment> \<open> Ppushl_i \<close> 
+    apply (unfold Let_def construct_rex_to_u8_def construct_modsib_to_u8_def)
+    subgoal 
+      using list_in_list_u8_list_of_u32_simp_sym [of imm  "(Suc (Suc pc))" l]
+      using length_u8_list_of_u32_eq_4
+      apply(auto simp add: x64_decode_def bitfield_insert_u8_def Let_def ireg_of_u8_def Suc3_eq_add_3 add.commute)
+    done
+
+  subgoal for dst
+    \<comment> \<open> Ppopl_i \<close> 
+    apply (unfold Let_def construct_rex_to_u8_def construct_modsib_to_u8_def)
+    apply (cases dst; auto simp add: x64_decode_def bitfield_insert_u8_def Let_def ireg_of_u8_def)
+    done
+
+  subgoal for dst src
+    \<comment> \<open> Ptestl_rr \<close>
+    apply (unfold Let_def construct_rex_to_u8_def construct_modsib_to_u8_def)
+    subgoal by (cases src; cases dst; auto simp add: x64_decode_def bitfield_insert_u8_def Let_def ireg_of_u8_def)
+    done
+
+  subgoal for dst src
+    \<comment> \<open> Ptestq_rr \<close>
+    apply (unfold Let_def construct_rex_to_u8_def construct_modsib_to_u8_def)
+    subgoal by (cases src; cases dst; auto simp add: x64_decode_def bitfield_insert_u8_def Let_def ireg_of_u8_def)
+    done
+
+
 *)
 end
